proof/correctness/Correctness_Mem.ec
@@ -5,7 +5,7 @@ require import AllCore List RealExp IntDiv.
 from Jasmin require import JModel.
 
 require import Array4 Array32 Array64 Array128 Array2144.
-require import RandomBytes XMSS_IMPL XMSS_IMPL_HOP1.
+require import RandomBytes XMSS_IMPL.
 require import Utils. (* valid_ptr predicate *)
 require import Termination.
 
@@ -129,26 +129,6 @@ qed.
 
 lemma _x_memcpy_u8u8_post (x : W8.t Array32.t) :
     phoare [M(Syscall)._x_memcpy_u8u8_32_32 : arg.`2 = x ==> res = x] = 1%r.
-proof.
-proc ; inline*.
-wp ; sp.
-while (* while invariante variante *)
-(0 <= to_uint i <= 32 /\ (forall (k : int), 0 <= k < to_uint i => (out1.[k] = in_01.[k]))) 
-(32 - to_uint i).
-  + auto => /> &hr i *; do split.
-      - smt(@W64).
-      - smt(@W64 pow2_64).
-      - move => k *. rewrite get_setE; 1:smt(@W64). case (k = to_uint i{hr}).
-           * move => * /#. 
-           * move => *. admit.
-      - smt(@W64 pow2_64).
-  + skip => /> &hr *. split; 1:smt(). progress.
-      - smt(@W64).
-      - rewrite tP. smt.
-qed.
-
-lemma _x_memcpy_u8u8_post_hop1 (x : W8.t Array32.t) :
-    phoare [M_Hop1(Syscall)._x_memcpy_u8u8_32_32 : arg.`2 = x ==> res = x] = 1%r.
 proof.
 proc ; inline*.
 wp ; sp.
